src/dvspec/dafny/commons.dfy
@@ -227,6 +227,12 @@ module CommonFunctions{
 
     lemma {:axiom} hash_tree_root_properties<T>()
     ensures forall d1: T, d2: T :: hash_tree_root(d1) == hash_tree_root(d2) ==> d1 == d2
+    
+    lemma {:axiom} exists_att_data_for_every_slashingDBattestaion()
+    ensures forall r: SlashingDBAttestation :: 
+                exists data: AttestationData :: 
+                    r.signing_root == Some(hash_tree_root(data))
+
 
 
     function getMessagesFromMessagesWithRecipient<M>(mswr: set<MessaageWithRecipient<M>>): set<M>
@@ -496,6 +502,88 @@ module CommonFunctions{
         var att_data: AttestationData :|  a.signing_root == Some(hash_tree_root(att_data));
 
         att_data.slot
+    }
+
+/*  // TODO: Prove post-condition
+    method get_slashing_db_attestations_before_slot_s(
+        db: set<SlashingDBAttestation>,
+        s: Slot
+    ) returns (S: set<SlashingDBAttestation>)
+    requires ( forall r: SlashingDBAttestation | r in db :: 
+                    ( exists att_data: AttestationData ::  r.signing_root == Some(hash_tree_root(att_data))
+                    )
+             )
+    ensures ( forall a | a in S :: get_slot_from_slashing_db_attestation(a) < s)
+    {           
+        if db == {} 
+        {
+            S := {};
+            assert ( forall a | a in S :: get_slot_from_slashing_db_attestation(a) < s);
+        }
+        else 
+        {                
+            var a: SlashingDBAttestation :| a in db;
+            var T := get_slashing_db_attestations_before_slot_s(db - {a}, s);
+            assert ( forall a | a in T :: get_slot_from_slashing_db_attestation(a) < s);
+            if get_slot_from_slashing_db_attestation(a) < s 
+            {                
+                S := { a } + T;
+                assert ( forall a | a in S :: get_slot_from_slashing_db_attestation(a) < s);
+            }
+            else 
+            {
+                S := T;
+                assert ( forall a | a in S :: get_slot_from_slashing_db_attestation(a) < s);
+            }                    
+        }
+*/
+
+    ghost method get_slashing_db_attestations_before_slot_s(
+        db: set<SlashingDBAttestation>,
+        s: Slot
+    ) returns (S: set<SlashingDBAttestation>)
+    requires ( forall r: SlashingDBAttestation | r in db :: 
+                    ( exists att_data: AttestationData ::  r.signing_root == Some(hash_tree_root(att_data))
+                    )
+             )
+    ensures ( forall r | r in S :: 
+                            && ( exists data: AttestationData ::  r.signing_root == Some(hash_tree_root(data)) )
+                            && get_slot_from_slashing_db_attestation(r) < s)
+    ensures ( forall r | r in db && r !in S :: 
+                            && ( exists data: AttestationData ::  r.signing_root == Some(hash_tree_root(data)) )
+                            && get_slot_from_slashing_db_attestation(r) >= s)
+    {
+        S := {};
+        var unchecked := db;
+        var checked := {};
+        
+        while unchecked != {}        
+        invariant unchecked + checked == db
+        invariant ( forall r: SlashingDBAttestation | r in S :: 
+                                && ( exists data: AttestationData ::  r.signing_root == Some(hash_tree_root(data)) )
+                                && get_slot_from_slashing_db_attestation(r) < s )
+        invariant ( forall r: SlashingDBAttestation | r in checked && r !in S ::
+                                && ( exists data: AttestationData ::  r.signing_root == Some(hash_tree_root(data)) )
+                                && get_slot_from_slashing_db_attestation(r) >= s )                            
+        decreases |unchecked|
+        {
+            var a: SlashingDBAttestation :| a in unchecked;
+            unchecked := unchecked - {a};
+            checked := checked + {a};
+
+            hash_tree_root_properties<AttestationData>();
+            var att_data: AttestationData :| a.signing_root == Some(hash_tree_root(att_data));
+            if att_data.slot < s
+            {
+                S := S + {a};
+            }
+            else 
+            {
+                S := S;
+            }            
+        }             
+
+        return S;
     }
 
     // Construct a slashing DB attestation for a given attestastion 
